theories/iris/logrel/iris_fundamental_host.v
@@ -1,0 +1,107 @@
+From iris.program_logic Require Import language.
+From iris.proofmode Require Import base tactics classes.
+From iris.base_logic Require Export gen_heap ghost_map proph_map na_invariants.
+From iris.base_logic.lib Require Export fancy_updates.
+From iris.algebra Require Import list.
+From iris.prelude Require Import options.
+
+Require Export iris iris_locations iris_properties iris_atomicity stdpp_aux.
+Require Export iris_rules.
+Require Export datatypes host operations properties opsem typing.
+Require Export iris_logrel iris_fundamental_helpers.
+
+Import uPred.
+
+Section fundamental.
+  Context `{!wasmG Σ, !logrel_na_invs Σ, !host_program_logic Σ}.
+
+    
+  Lemma typing_local_host C es τ1 τ2 τs hctx hl :
+    (∀ C es τ, be_typing C es τ -> ⊢ semantic_typing C (to_e_list es) τ) ->
+    (tc_label C) = [] ∧ (tc_return C) = None ->
+    be_typing (upd_local_label_return C (τ1 ++ τs) [τ2] (Some τ2)) es (Tf [] τ2) ->
+    ⊢ semantic_typing_local C hl es τs (Tf τ1 τ2) hctx.
+  Proof.
+    intros be_fundamental Hnil Htyping.
+    iSplit;[auto|].
+    iIntros (i) "#Hi #Hhcalls #Hhreturn". iIntros (f vs) "Hf Hown #Hv".
+    apply be_fundamental in Htyping.
+    iDestruct (Htyping) as "Ht".
+    iDestruct (interp_instance_change_label [τ2] with "Hi") as "Hi'".
+    iDestruct (interp_instance_change_return (Some τ2) with "Hi'") as "Hi''".
+    iDestruct (interp_instance_change_local τ1 with "Hi''") as "Hi_final".
+    iSpecialize ("Ht" $! _ (LH_rec [] (length τ2) [] (LH_base [] []) []) with "[$Hi_final] []").
+    { unfold interp_ctx. iSimpl. repeat (iSplit;[by auto|]).
+      iSplit =>//. unfold interp_ctx_continuation.
+      iSimpl. iExists _,_,_,_,_,(LH_base [] []). iSplit;[eauto|].
+      repeat (iSplit;[by auto|]). iModIntro.
+      iIntros (v f') "#Hv' [Hf' Hfv']".
+      iExists τ2. rewrite app_nil_l !app_nil_r.
+      iApply wp_value;[done|].
+      iSplitR;[|iExists _;iFrame].
+      iLeft. iFrame "Hv'". }
+
+    destruct (iris.to_val [AI_local (length τ2) {| f_locs := vs; f_inst := i |}
+                                    [AI_label (length τ2) [] (to_e_list es)]]) eqn:Hetov.
+    { apply to_val_local_inv in Hetov as Heq.
+      destruct Heq as [tf [h [w [vh Heq]]]]. subst v.
+      apply to_val_call_host_rec_local in Hetov as Heq.
+      destruct Heq as [LI [Heq HLI]].
+      simpl in Heq. inversion Heq. subst.
+      apply to_val_call_host_label_inv in HLI as Heq'.
+      destruct Heq' as [vh' [Heq' Hvh']]. subst.
+      apply to_es_list_llfill_contr in Hvh'. done.
+    }
+
+    unfold interp_expression_closure.
+    iApply wp_host_bind.
+    iApply (wp_wand _ _ _ ((λ vs0,
+               (interp_val τ2 vs0
+                ∨ interp_call_host_cls hl τ2 vs0) ∗
+               ↪[frame]f ∗ na_own logrel_nais ⊤)%I) with "[-]").
+    { iApply (wp_frame_bind with "Hf");[auto|].
+      iIntros "Hf".
+      iApply wp_wasm_empty_ctx.
+      iApply wp_label_push_nil.
+      iApply wp_label_bind.
+      iDestruct ("Ht" $! _ (immV []) with "[$Hf Hown] []") as "Hcont".
+      { iExists _. iFrame. iSplit;eauto. }
+      { iRight. iExists _. iSplit;eauto. }
+      iSimpl in "Hcont". unfold interp_expression.
+      iApply (wp_wand with "Hcont").
+      iClear "Ht".
+      iIntros (v) "[Hv' Hf0]".
+      iDestruct "Hf0" as (f0) "[Hf0 Hf0v]".
+      iDestruct "Hv'" as "[[-> | Hv'] | [Hbr | [Hret | Hch] ]]";simpl language.of_val.
+      { iApply (local_host_trap with "[$] [$]"). }
+      { iApply (local_host_val with "[$] [$] [$]"). }
+      { iApply (local_host_br with "[$] [$] [$]"). }
+      { iApply (local_host_ret with "[$] [$] [$]"). }
+      { iApply (local_host_call with "[$] [$] [$]"). }
+    }
+    
+    iIntros (v) "[[#Hres | #Hres] [Hf Hown]]".
+    { iApply ("Hhreturn" with "Hres Hown Hf"). }
+    { iAssert (▷ interp_call_host_cls hl τ2 v)%I with "Hres" as "Hres'";iClear "Hres".
+      iRevert "Hres'". iLöb as "IH"
+    forall (v);iIntros "#Hres".
+
+      rewrite fixpoint_interp_call_host_cls_eq. iApply fupd_wp_host.
+      iDestruct "Hres" as (? ? ? ? ? ?) "[>%Heq [>%Htf [>%Hin [>%Hb [>#Hval Hres]]]]]".
+      iModIntro.
+      rewrite Heq. simpl iris.of_val.
+      iDestruct (big_sepL_elem_of with "Hhcalls") as "Hh";eauto.
+      destruct tf. simplify_eq. unfold interp_closure_host.
+      iApply ("Hh" with "Hval Hown Hf").
+      iNext. iIntros (v2) "#Hv2 Hown Hf".
+
+      iApply wp_host_bind.
+      iDestruct ("Hres" with "Hv2 Hf Hown") as "Hcont".
+      iApply (wp_wand with "Hcont").
+      iIntros (v) "[[Hw|#Hw] [Hown Hf]]".
+      { iApply ("Hhreturn" with "Hw Hf Hown"). }
+      { iApply ("IH" with "Hown Hf"). iModIntro. iNext. iFrame "Hw". }
+    }
+  Qed.
+  
+End fundamental.
